src/JSON_Type.v
@@ -1,10 +1,37 @@
 Require Import String Maps.
 
+Require Import List.
+
+
 Inductive JSON :=
-| JSON_Object     : MapC string InnerJSON -> JSON
+| JSON_Object   : Map string JSON -> JSON
+| JSON_Array    : list JSON -> JSON
+| JSON_String   : string -> JSON
+| JSON_Boolean  : bool -> JSON.
+
+
+(*
+Inductive JSON :=
+| JSON_Object     : Map string InnerJSON -> JSON
 
 with InnerJSON :=
 | InJSON_Object   : JSON -> InnerJSON
 | InJSON_Array    : list InnerJSON -> InnerJSON
 | InJSON_String   : string -> InnerJSON
 | InJSON_Boolean  : bool -> InnerJSON.
+
+*)
+
+Definition depth_js_array (ls:list JSON) (f:JSON -> nat) : nat := 
+    fold_right (fun js acc => max acc (f js)) 0 ls.
+
+Definition depth_js_map (m: Map string JSON) (f:JSON -> nat) : nat := 
+    fold_right (fun pr acc => max acc (f (snd pr))) 0 m.
+
+Fixpoint JSON_depth (js:JSON) : nat := 
+    match js with
+    | JSON_Boolean _ => 1 
+    | JSON_String _ => 1 
+    | JSON_Array ls => 1 + depth_js_array ls JSON_depth
+    | JSON_Object m => 1 + depth_js_map m JSON_depth
+    end.
