src/Extraction_Cvm_Cake.v
@@ -1,0 +1,46 @@
+(*  Configuring and invoking custom CakeML code extraction.  *)
+
+Require Extraction.
+
+Require Import Term_Defs Term_Defs_Core IO_Stubs AM_Monad Cvm_Monad Cvm_Impl.
+(* Require Import CopParser. *)
+
+Require Import Manifest_Generator Session_Config_Compiler.
+
+Require Import AM_Helpers Server_AM Client_AM.
+
+Require Import Manifest_Generator_Union Manifest_JSON Flexible_Mechanisms.
+
+Require Import AppraisalSummary.
+
+Require Import List.
+Import ListNotations.
+
+Require Import Concrete_Extractables.
+
+Require Import ExtrCakeMLNativeString.
+
+Extraction Language CakeML. (* OCaml. *) 
+
+Extraction Implicit parallel_vm_thread [2 3 4].
+Extraction Implicit do_wait_par_thread [2 3 4].
+
+Extract Constant sig_params => "( undefined () )".
+Extract Constant hsh_params => "( undefined () )".
+Extract Inlined Constant Nat.eqb => "(op=)".
+(* Extract Constant + => "add". *)
+(* Extract Constant Nat.add => "(+)". *)
+
+Separate Extraction 
+    full_flexible_mechanisms
+    build_cvm session_config_compiler 
+		handle_AM_request end_to_end_mangen
+    concrete_Jsonifiable_Manifest
+    concrete_Jsonifiable_ASP_Compat_MapT
+    concrete_Jsonifiable_Attestation_Session
+    concrete_Jsonifiable_Term
+    concrete_Jsonifiable_EvidenceT
+    concrete_Jsonifiable_GlobalContext
+    Jsonifiable_Term_Plc_list
+    test_app_summary_compute_json
+    am_client_app_summary.
