src/Interface_Strings_Vars.v
@@ -1,0 +1,33 @@
+Require Import String.
+
+(* Interface string Values *)
+Definition STR_REQ_PLC : string := "REQ_PLC".
+Definition STR_TERM : string := "TERM".
+Definition STR_RAWEV : string := "RAWEV".
+Definition STR_SUCCESS : string := "SUCCESS".
+Definition STR_PAYLOAD : string := "PAYLOAD".
+Definition STR_EVIDENCE : string := "EVIDENCE".
+
+Definition STR_ACTION : string := "ACTION".
+Definition STR_TYPE : string := "TYPE".
+
+Definition STR_RUN : string := "RUN".
+Definition STR_NEGOTIATE : string := "NEGOTIATE".
+Definition STR_APPRAISE : string := "APPRAISE".
+Definition STR_REQUEST : string := "REQUEST".
+Definition STR_RESPONSE : string := "RESPONSE".
+
+Definition STR_ATTEST_SESS : string := "ATTESTATION_SESSION".
+
+(* ASP String Admits *)
+Definition STR_ASP : string := "ASP".
+Definition STR_ASP_RUN : string := "ASP_RUN".
+Definition STR_ASP_ID : string := "ASP_ID".
+Definition STR_ASP_ARGS : string := "ASP_ARGS".
+Definition STR_ASP_PLC : string := "ASP_PLC".
+Definition STR_ASP_TARG_ID : string := "ASP_TARG_ID".
+
+Definition STR_Session_Plc : string := "Session_Plc".
+Definition STR_Plc_Mapping : string := "Plc_Mapping".
+Definition STR_PubKey_Mapping : string := "PubKey_Mapping".
+Definition STR_Session_Context : string := "Session_Context".
